proof/correctness/avx2/1024/MLKEM_InnerPKE_avx2_new.ec
@@ -7,6 +7,7 @@ require import AVX2_Ops W16extra.
 from JazzEC require import Jkem_avx2.
 require import MLKEM_PolyVec_avx2.
 require import MLKEM_Poly_avx2.
+require import MLKEM_Poly_avx2_circuit MLKEM_Poly_avx2_circuit_1024 MLKEM_PolyVec_avx2_circuit.
 require import NTT_avx2 NTT_avx2_poly.
 require import MLKEM_W16_Rep.
 require import MLKEM1024_prelude.
@@ -324,21 +325,29 @@ have H := polyvec_pointwise_acc_corr_avx_ph a_ref b_ref
 + done.
 + by move => k kb; rewrite /R /(&+) /= map2E !initiE //= map2E !initiE //= map2E !initiE //=.
 conseq H.
-+ move => &hr [Hva [Habnd [Hvb [Hbbnd [Halift [Hblift [Hab Hbb]]]]]]]; do split => //;
-    rewrite /A0 /A1 /A2 /A3 /B0 /B1 /B2 /B3 ?Hva ?Hvb /lift_polyvec;
-    rewrite tP => k kb; rewrite getvE; smt(Vector.offunvE).
+move => &hr [Hva [Habnd [Hvb [Hbbnd [Halift [Hblift [Hab Hbb]]]]]]]; do split => //.
+by rewrite /A0 Hva /lift_polyvec KVec.initiE; smt(kvec_val).
+by rewrite /A1 Hva /lift_polyvec KVec.initiE; smt(kvec_val).
+by rewrite /A2 Hva /lift_polyvec KVec.initiE; smt(kvec_val).
+by rewrite /A3 Hva /lift_polyvec KVec.initiE; smt(kvec_val).
+by rewrite /B0 Hvb /lift_polyvec KVec.initiE; smt(kvec_val).
+by rewrite /B1 Hvb /lift_polyvec KVec.initiE; smt(kvec_val).
+by rewrite /B2 Hvb /lift_polyvec KVec.initiE; smt(kvec_val).
+by rewrite /B3 Hvb /lift_polyvec KVec.initiE; smt(kvec_val).
 move => &hr Hpre result; have ->: nttunpack (scale (ntt (dotpw va vb)) (incoeff 169)) = nttunpack R; last done.
-congr; rewrite mulvec.
+congr; rewrite dotpwE mulvec kvec_val.
+rewrite (Big.BAdd.big_int_recl 3) // (Big.BAdd.big_int_recl 2) // (Big.BAdd.big_int_recl 1) // (Big.BAdd.big_int_recl 0) // Big.BAdd.big_geq //=.
 rewrite !add_comm_ntt !nttK.
-have HEva : forall i, 0 <= i < 4 => tofunv va i = va.[i]%Vector by smt().
-have HEvb : forall i, 0 <= i < 4 => tofunv vb i = vb.[i]%Vector by smt().
-rewrite /R /P0 /P1 /P2 /P3 /A0 /A1 /A2 /A3 /B0 /B1 /B2 /B3 /PolyVec.nttv /mapv
-        /scale /(&+) tP => k kb.
+rewrite !poly2algE.
+smt(kvec_val). smt(kvec_val). smt(kvec_val). smt(kvec_val). smt(kvec_val). smt(kvec_val). smt(kvec_val). smt(kvec_val).
+rewrite /R /P0 /P1 /P2 /P3 /A0 /A1 /A2 /A3 /B0 /B1 /B2 /B3.
+rewrite nttZero !nttvE.
+smt(kvec_val). smt(kvec_val). smt(kvec_val). smt(kvec_val). smt(kvec_val). smt(kvec_val). smt(kvec_val). smt(kvec_val).
+rewrite /scale /(&+) tP => k kb.
 rewrite !mapiE //= !map2iE //= !mapiE //=.
-rewrite !mapvE /= !getvE !offunvE //=.
-rewrite (HEva 0) // (HEva 1) // (HEva 2) // (HEva 3) //
-        (HEvb 0) // (HEvb 1) // (HEvb 2) // (HEvb 3) //.
-by  ring.
+rewrite /zero Array256.createiE 1:/#.
+have ->: incoeff 0 = Zq.zero by done.
+by ring.
 qed.
 
 
@@ -351,17 +360,17 @@ proof. by rewrite -nttpackv_lift packvK. qed.
 lemma lift_polyvec_nttpackv_add (X Y Z : W16.t Array1024.t) :
   (forall k, 0 <= k < 1024 =>
      (lift_array1024 Z).[k] = (lift_array1024 X).[k] + (lift_array1024 Y).[k]) =>
-  lift_polyvec (nttpackv Z) = (lift_polyvec (nttpackv X) + lift_polyvec (nttpackv Y))%Vector.
+  lift_polyvec (nttpackv Z) = (lift_polyvec (nttpackv X) + lift_polyvec (nttpackv Y)).
 proof.
 move => Hpw.
-apply eq_vectorP => j Hj.
-rewrite /lift_polyvec.
-rewrite !KMatrix.Vector.offunvE 1..2:/# /=.
-rewrite -!getvE.
-rewrite /(&+).
+have kv := kvec_val.
+apply KVec.tP => j Hj.
+rewrite polyvec_addE; 1: smt(kvec_val).
+rewrite /lift_polyvec !KVec.initiE; 1,2,3: smt(kvec_val).
+simplify.
 rewrite tP => k Hk.
-rewrite Array256.map2iE 1:/# /=.
-rewrite /lift_array256 /subarray256 !mapiE 1:/# /= !initiE 1:/# /=.
+rewrite /(&+) Array256.map2iE 1:/# /=.
+rewrite /lift_array256 /subarray256 !mapiE //= !initiE //=.
 have peel : forall (W : W16.t Array1024.t),
             (nttpackv W).[256*j + k] = W.[256*j + nttpack_idx.[k]].
 + move => W; rewrite /nttpackv initiE 1:/# /= initiE 1:/# /=.
@@ -379,49 +388,49 @@ have peel : forall (W : W16.t Array1024.t),
   - rewrite ifF 1:/# ifF 1:/# ifF 1:/# /nttpack initiE /=; 1: smt(nttpack_bnd Array256.allP mem_iota).
     rewrite /subarray256 initiE /=; 1: smt(nttpack_bnd Array256.allP mem_iota).
   by rewrite initiE /=; 1: smt(nttpack_bnd Array256.allP mem_iota).
-rewrite peel.
-rewrite !getvE !offunvE /=; 1..2: smt(nttpack_bnd Array256.allP mem_iota).
-rewrite !mapiE /=; 1..2: smt(nttpack_bnd Array256.allP mem_iota).
-pose a := NTT_AVX_j.incoeffW16 Z.[256 * j + nttpack_idx.[k]].
-rewrite !initiE /=; 1,2: smt(nttpack_bnd Array256.allP mem_iota).
-rewrite peel /a.
+rewrite !peel.
 move: (Hpw (256*j + nttpack_idx.[k]) _); first smt(nttpack_bnd Array256.allP mem_iota).
 rewrite /lift_array1024 !mapiE /=; 1..3: smt(nttpack_bnd Array256.allP mem_iota).
 smt().
 qed.
 
-lemma lift_array1024_unlift_ofipolyvec (vi : int Array1024.t) :
+lemma encode12_vec_tobytes_bridge (X : W16.t Array1024.t) :
+  encode12_vec (toipolyvec (lift_polyvec X))
+  = BytesPKVec.init (fun i =>
+      (Array1536.of_list W8.zero
+         (ByteEncode 12 (to_list (map asint (lift_array1024 X))))).[i]).
+proof.
+have Hk1024 : 256 * Parameters.kvec = 1024 by smt(kvec_val).
+have H1536 : 384 * Parameters.kvec = 1536 by smt(kvec_val).
+rewrite /encode12_vec toipolivec_lift.
+have ->: to_list (IPVec.init (fun (idx : int) => asint (lift_array1024 X).[idx]))
+       = to_list (map asint (lift_array1024 X)).
++ apply (eq_from_nth witness).
+  + rewrite IPVec.size_to_list Array1024.size_to_list; smt().
+  move => i; rewrite IPVec.size_to_list => Hi.
+  have Hi1024 : 0 <= i < 1024 by rewrite -Hk1024; exact Hi.
+  rewrite IPVec.get_to_list Array1024.get_to_list IPVec.initiE 1:/#.
+  simplify.
+  rewrite Array1024.mapiE 1:/#.
+  by rewrite /lift_array1024 Array1024.mapiE 1:/# Array1024.mapiE 1:/#.
+apply BytesPKVec.tP => k Hk.
+have Hk1536 : 0 <= k < 1536 by rewrite -H1536; exact Hk.
+by rewrite get_of_list 1:/# initiE 1:/# /= get_of_list 1:/#.
+qed.
+
+lemma lift_array1024_unlift_ofipolyvec (vi : ipolyvec) :
   all (fun i => 0 <= i < 32768) vi =>
-  lift_array1024 (unlift_polyvec (ofipolyvec vi)) = map incoeff vi.
+  lift_array1024 (unlift_polyvec (ofipolyvec vi)) = Array1024.init (fun k => incoeff vi.[k]).
 proof.
 rewrite allP => Hbnd.
+have kv := kvec_val.
 rewrite /lift_array1024 /unlift_polyvec /ofipolyvec tP => k kb.
-rewrite !mapiE //= initiE 1://;beta.
-rewrite !setvE;beta;rewrite !offunvK /vclamp; beta.
-rewrite offunvE 1:/# /kvec;beta.
-have Hkr : k = 256 * (k %/ 256) + k %% 256 by smt().
-have Hkdiv : k %/ 256 = 0 \/ k %/ 256 = 1 \/ k %/ 256 = 2 \/ k %/ 256 = 3 by smt().
-case Hkdiv => [H0 | [H0 | [H0 | H0]]]; rewrite H0.
-+ rewrite ifF 1:/# ifT 1:/# ifF 1:/# ifT 1:/# ifF 1:/# ifT 1:/# ifT 1:/#.
-  rewrite mapiE 1:/# /subarray256 initiE 1:/#;beta.
-  rewrite of_sintK Montgomery16.smod_small.
-  + have := as_sint_range (incoeff vi.[256 * 0 + k %% 256]); smt(qE).
-  by rewrite as_sintK; have -> : 256 * 0 + k %% 256 = k by move : Hkr; smt().
-+ rewrite ifF 1:/# ifT 1:/# ifF 1:/# ifT 1:/# ifT 1:/#.
-  rewrite mapiE 1:/# /subarray256 initiE 1:/#;beta.
-  rewrite of_sintK Montgomery16.smod_small.
-  + have := as_sint_range (incoeff vi.[256 * 1 + k %% 256]); smt(qE).
-  by rewrite as_sintK; have -> : 256 * 1 + k %% 256 = k by move : Hkr; smt().
-+ rewrite ifF 1:/# ifT 1:/# ifT 1:/#.
-  rewrite mapiE 1:/# /subarray256 initiE 1:/#;beta.
-  rewrite of_sintK Montgomery16.smod_small.
-  + have := as_sint_range (incoeff vi.[256 * 2 + k %% 256]); smt(qE).
-  by rewrite as_sintK; have -> : 256 * 2 + k %% 256 = k by move : Hkr; smt().
-+ rewrite ifT 1:/#.
-  rewrite mapiE 1:/# /subarray256 initiE 1:/#;beta.
-  rewrite of_sintK Montgomery16.smod_small.
-  + have := as_sint_range (incoeff vi.[256 * 3 + k %% 256]); smt(qE).
-  by rewrite as_sintK; have -> : 256 * 3 + k %% 256 = k by move : Hkr; smt().
+rewrite Array1024.mapiE 1:/# /= Array1024.initiE 1:/# /= KVec.initiE 1:/# /= mapiE 1:/# /= /subarray256 initiE 1:/# /=.
+rewrite Array1024.initiE 1:/# /=.
+have ->: 256 * (k %/ 256) + k %% 256 = k by smt().
+rewrite of_sintK Montgomery16.smod_small.
++ have := as_sint_range (incoeff vi.[k]); smt(qE).
+by rewrite as_sintK.
 qed.
 
 lemma ntt_dotp_invnttv (s u : PolyVec.polyvec) :
@@ -432,20 +441,19 @@ proof. by rewrite dotpwE comm_ntt_dotp nttK. qed.
    the (i,j) coefficient block of the original polymat. 1024 variant. *)
 lemma lift_polyvec_subarray1024_unlift_matrix (a : polymat) (i j : int) :
   0 <= i < 4 => 0 <= j < 4 =>
-  (lift_polyvec (subarray1024 (unlift_matrix a) i)).[j]%Vector = a.[i, j]%Matrix.
+  (lift_polyvec (subarray1024 (unlift_matrix a) i)).[j] = a.[(i, j)].
 proof.
 move => Hi Hj.
-rewrite /lift_polyvec offunvE 1:/# /= /lift_array256 tP => k Hk.
+have kv := kvec_val.
+rewrite /lift_polyvec KVec.initiE 1:/# /= /lift_array256 tP => k Hk.
 rewrite /subarray256 /subarray1024 mapiE 1:/# /= initiE 1:/# /= initiE 1:/# /=.
 rewrite /unlift_matrix initiE 1:/# /=.
 have ->: (1024 * i + (256 * j + k)) %/ 1024 = i by smt().
 have ->: (1024 * i + (256 * j + k)) %% 1024 = 256 * j + k by smt().
 have ->: (256 * j + k) %/ 256 = j by smt().
 have ->: (1024 * i + (256 * j + k)) %% 256 = k by smt().
-rewrite /to_sint /= modz_small; 1: by smt(rg_asint qE).
-rewrite /smod /=.
-have ->: (32768 <= asint a.[i, j]%Matrix.[k]) = false by smt(rg_asint qE).
-by rewrite /= asintK.
+rewrite W16.to_sintE W16.of_uintK /smod /=.
+by smt(asintK rg_asint qE).
 qed.
 
 lemma frommont_cancels_at_slot (rr0 rr1 : W16.t Array256.t) (X : poly) :
@@ -519,11 +527,12 @@ lemma kg_loop_post_to_target (pkpv : W16.t Array1024.t) (mm : PolyVec.polyvec) :
   lift_polyvec (nttpackv pkpv) = mm.
 proof.
 move => Hslots.
-rewrite eq_vectorP => j jb.
-have := Hslots j; rewrite jb /= getvE => Hslotsj.
-rewrite -(nttunpackK (mm.[j])%Vector).
+apply KVec.tP => j jb.
+have Hslotsj := Hslots j _; first smt(kvec_val).
+rewrite -(nttunpackK mm.[j]).
 rewrite -Hslotsj.
-rewrite /lift_polyvec offunvE 1:/# /=.
+rewrite /lift_polyvec KVec.initiE 1:/# /=.
+have kv := kvec_val.
 have lift_subarrayE : forall (X : W16.t Array1024.t) (jj : int),
   0 <= jj < 4 =>
   lift_array256 (subarray256 X jj) =
@@ -641,17 +650,12 @@ lemma ntt_dotp_row_eq_ntt_mmul (a : polymat) (sv : W16.t Array1024.t) (i : int) 
   = (ntt_mmul a (lift_polyvec (nttpackv sv))).[i]%PolyVec.
 proof.
 move => Hi.
+have kv := kvec_val.
 rewrite ntt_dotp_invnttv nttvK.
 rewrite (nttpackv_subarray1024_nttunpackm (unlift_matrix a) i _) //=.
-rewrite /ntt_dotp !getvE !(lift_polyvec_subarray1024_unlift_matrix a i _ _) //=.
-case (i = 0) => Hi0.
-+ by rewrite Hi0 /= !offunvE //= /ntt_mmul !setvE !offunvE //= offunvK /vclamp ifT 1:/# /= offunvK /vclamp ifT 1:/# /= offunvK /vclamp ifT 1:/# /= !getvE /= !getmE /lift_polyvec !offunvE //=.
-case (i = 1) => Hi1.
-+ by rewrite Hi1 /= !offunvE //= /ntt_mmul !setvE !offunvE //= offunvK /vclamp ifT 1:/# /= offunvK /vclamp ifT 1:/# /= !getvE /= !getmE /lift_polyvec !offunvE //=.
-case (i = 2) => Hi2.
-+ by rewrite Hi2 /= !offunvE //= /ntt_mmul !setvE !offunvE //= offunvK /vclamp ifT 1:/# /= !getvE /= !getmE /lift_polyvec !offunvE //=.
-have -> : (i = 3) by smt().
-by rewrite !offunvE //= /ntt_mmul !setvE !offunvE //= !getvE /= !getmE /lift_polyvec !offunvE //=.
+rewrite ntt_dotpE /ntt_mmul KVec.initiE 1:/# /= nttsum_big /range /=.
+apply Big.BAdd.eq_big_seq => j /mem_iota jb /=.
+by rewrite (lift_polyvec_subarray1024_unlift_matrix a i j _ _); smt(kvec_val).
 qed.
 
 lemma poly_add2_avx_ll : islossless Jkem_avx2.M._poly_add2.
@@ -669,23 +673,71 @@ wp; call poly_basemul_avx_ll; auto; smt().
 qed.
 
 
+lemma decode_vec_c1_bridge (f : int -> W8.t) :
+  decode_vec (BytesCtVec.init f) = Circuit_sem_1024.decode11_vec (Array1408.init f).
+proof.
+have Hdu : Parameters.du = 11 by smt(Parameters.param_sets kvec_val).
+have Hsz : 32 * Parameters.du * Parameters.kvec = 1408 by smt(Parameters.param_sets kvec_val).
+rewrite /decode_vec Hdu; congr; congr.
+apply (eq_from_nth witness).
++ rewrite BytesCtVec.size_to_list Array1408.size_to_list; smt().
+move => i; rewrite BytesCtVec.size_to_list => Hi.
+have Hi1408 : 0 <= i < 1408 by smt().
+by rewrite BytesCtVec.get_to_list Array1408.get_to_list initiE 1:/# initiE 1:/#.
+qed.
+
+lemma decode_poly_c2_bridge (f : int -> W8.t) :
+  decode_poly (BytesPoly.init f) = Circuit_sem_1024.decode5 (Array160.init f).
+proof.
+have Hdv : Parameters.dv = 5 by smt(Parameters.param_sets kvec_val).
+have Hsz : 32 * Parameters.dv = 160 by smt(Parameters.param_sets kvec_val).
+rewrite /decode_poly Hdv; congr; congr.
+apply (eq_from_nth witness).
++ rewrite BytesPoly.size_to_list Array160.size_to_list; smt().
+move => i; rewrite BytesPoly.size_to_list => Hi.
+have Hi160 : 0 <= i < 160 by smt().
+by rewrite BytesPoly.get_to_list Array160.get_to_list initiE 1:/# initiE 1:/#.
+qed.
+
+
+lemma frombytes12_decode_bridge (f : int -> W8.t) :
+  Array1024.of_list (incoeff 0)
+    (map incoeff (ByteDecode 12 (to_list (Array1536.init f))))
+  = Array1024.init (fun kk => incoeff (decode12_vec (BytesPKVec.init f)).[kk]).
+proof.
+have Hd : size (ByteDecode 12 (to_list (Array1536.init f))) = 1024.
++ rewrite (size_decode 4 12 (to_list (Array1536.init f))) //; smt(Array1536.size_to_list).
+have Hbytes : to_list (Array1536.init f) = to_list (BytesPKVec.init f).
++ apply (eq_from_nth witness); 1: (rewrite Array1536.size_to_list BytesPKVec.size_to_list; smt(kvec_val)).
+  move => i; rewrite Array1536.size_to_list => Hi.
+  rewrite Array1536.get_to_list BytesPKVec.get_to_list.
+  rewrite Array1536.initiE //= BytesPKVec.initiE //=.
+  smt(kvec_val).
+apply Array1024.tP => k Hk.
+rewrite get_of_list 1:/# (nth_map 0).
++ by rewrite Hd.
+rewrite Array1024.initiE //= /decode12_vec get_of_list.
++ smt(kvec_val).
+by rewrite Hbytes.
+qed.
+
 lemma mlkem_correct_enc_avx2_op _pkp :
   equiv [Jkem_avx2.M.__indcpa_enc ~ InnerPKE_Op.enc_derand :
     msgp{1} = m{2} /\ pk{1} = _pkp /\
     noiseseed{1} = r{2} /\
-    pk{2}.`1 = Array1536.init (fun i => pk{1}.[i]) /\
+    pk{2}.`1 = BytesPKVec.init (fun i => pk{1}.[i]) /\
     pk{2}.`2 = Array32.init (fun i => pk{1}.[i+1536])
     ==>
     let (c1,c2) = res{2} in
-    c1 = Array1408.init (fun i => res{1}.[i]) /\
-    c2 = Array160.init (fun i => res{1}.[i+1408])].
+    c1 = BytesCtVec.init (fun i => res{1}.[i]) /\
+    c2 = BytesPoly.init (fun i => res{1}.[i+1408])].
 proof.
 proc => /=.
 
 (* === Step 1: pkpv decode + publicseed extraction + message decompress. === *)
 seq 14 9 : (#pre /\
             publicseed{1} = rho{2} /\
-            lift_array1024 pkpv{1} = nttunpackv (map incoeff (decode12_vec pk{2}.`1)) /\
+            lift_array1024 pkpv{1} = nttunpackv (Array1024.init (fun kk => incoeff (decode12_vec pk{2}.`1).[kk])) /\
             pos_bound1024_cxq pkpv{1} 0 1024 2 /\
             that{2} = ofipolyvec (decode12_vec pk{2}.`1) /\
             lift_array256 k{1} = decompress_poly 1 (decode1 m{2}) /\
@@ -710,9 +762,10 @@ seq 14 9 : (#pre /\
        split; 1: smt().
        move => publicseed_L w_L; split; 1: smt().
        move => Hncond Hwl Hwh Hcov result0 Hlift0 Hbnd0.
-       split; last by rewrite Hpk1.
-       apply Array32.tP => k Hk.
-       rewrite Hpk2 initiE 1:/# /=; smt().
+       split.
+       + apply Array32.tP => k Hk.
+         rewrite Hpk2 initiE 1:/# /=; smt().
+       rewrite Hlift Hpk1; congr; apply frombytes12_decode_bridge.
 
 (* === Step 2: matrix gen, transposed. === *)
 seq 2 1 : (#pre /\
@@ -723,12 +776,10 @@ seq 2 1 : (#pre /\
        ecall {1} (_gen_matrix_avx2_sem publicseed{1} true).
        auto => /> &1 &2 ??????; do split.
        + congr;congr.
-         rewrite /H; apply eq_matrixP => i j [Hi Hj].
-          rewrite /nttm /invnttm !mapmE  !offunmE 1,2:/# /= /trmx offunmK /mclamp ifT 1:/#.
-          rewrite offunmE 1:/# /= nttK /=; by smt(offunmE).
-       + rewrite /H; apply eq_matrixP => i j [Hi Hj].
-          rewrite /nttm /invnttm !mapmE  !offunmE 1,2:/# /= /trmx offunmK /mclamp ifT 1:/#.
-          rewrite offunmE 1:/# /= nttK /=; by smt(offunmE).
+         apply eq_polymatP => i j Hi Hj.
+         rewrite trmxE 1,2:/# nttmE 1,2:/# trmxE 1,2:/# /H invnttmE 1,2:/# nttK //.
+       + apply eq_polymatP => i j Hi Hj.
+         rewrite nttmE 1,2:/# trmxE 1,2:/# /H invnttmE 1,2:/# nttK trmxE 1,2:/# //.
        + rewrite /pos_bound4096_cxq /nttunpackm => k kb.
          rewrite initiE 1:/# /=.
          (* TODO 1024: 4-way case-split (was 3-way in 768) *)
@@ -763,7 +814,7 @@ seq 2 1 : (#pre /\
 seq 6 0 : (#pre /\
            (forall i, 0 <= i < 4 =>
               lift_array256 (Array256.init (fun k => sp_0{1}.[256*i + k])) =
-                cbd2sample (Symmetric.PRF noiseseed{1} (W8.of_int i))) /\
+                samplePolyCBD (Symmetric.PRF noiseseed{1} (W8.of_int i))) /\
            signed_bound1024_cxq sp_0{1} 0 1024 1).
 +  sp 1 0.
   wp.
@@ -796,7 +847,7 @@ seq 6 0 : (#pre /\
 (* Step 4a: fill ep cleanly (4 polys) — mirrors Step 3 pattern. *)
 seq 6 0 : (#{/~forall i, 0 <= i < 4 =>
                 lift_array256 (Array256.init (fun k => sp_0{1}.[256*i + k])) =
-                  cbd2sample (Symmetric.PRF noiseseed{1} (W8.of_int i))}
+                  samplePolyCBD (Symmetric.PRF noiseseed{1} (W8.of_int i))}
             {/~signed_bound1024_cxq sp_0{1} 0 1024 1}pre /\
            lift_polyvec sp_0{1} = rv{2} /\
            lift_polyvec ep{1} = e1{2} /\
@@ -810,37 +861,37 @@ seq 6 0 : (#{/~forall i, 0 <= i < 4 =>
   have Hep_eq : e1{2} = (prg_enc_inner r{2}).`2 by smt().
   do split.
   + (* lift_polyvec sp_0 = rv{2} *)
-    have Hrv : forall i, 0 <= i < kvec => rv{2}.[i]%Vector = cbd2sample (PRF r{2} (W8.of_int i)).
+    have Hrv : forall i, 0 <= i < Parameters.kvec => rv{2}.[i] = samplePolyCBD (PRF r{2} (W8.of_int i)).
     + move => i Hi.
-      have ->: rv{2}.[i]%Vector = (prg_enc_inner r{2}).`1.[i]%Vector by rewrite Hrv_eq.
-      by rewrite /prg_enc_inner /= offunvE 1:/# /=.
-    rewrite eq_vectorP => i Hi.
-    rewrite Hrv 1:/# offunvE 1:/# /=.
-    have Hspi := Hsp_fa i _; first by smt().
+      have ->: rv{2}.[i] = (prg_enc_inner r{2}).`1.[i] by rewrite Hrv_eq.
+      by rewrite /prg_enc_inner /= KVec.initiE 1:/# /=.
+    apply KVec.tP => i Hi.
+    rewrite Hrv 1:/# /lift_polyvec KVec.initiE 1:/# /=.
+    have Hspi := Hsp_fa i _; first by smt(kvec_val).
     rewrite tP => k Hk.
     move: Hspi; rewrite /lift_array256 /subarray256 tP => /(_ k _); first by smt().
     by rewrite !mapiE 1:/# /=.
   + (* lift_polyvec ep = e1{2} *)
-    rewrite eq_vectorP => i Hi.
-    rewrite offunvE 1:/# /= /PRF.
+    apply KVec.tP => i Hi.
+    rewrite /lift_polyvec KVec.initiE 1:/# /= /PRF.
     rewrite /lift_array256 /subarray256 tP => k Hk.
     rewrite mapiE 1:/# /= initiE 1:/# /=.
     case (i = 0) => Ci0.
     + rewrite Ci0 /= initiE 1:/# /= initiE 1:/# /= initiE 1:/# /= initiE 1:/# /= ifF 1:/# ifF 1:/# ifF 1:/# ifT 1:/#.
       have := Hr1; rewrite /lift_array256 tP => /(_ k _); 1: smt(); rewrite mapiE 1:/# /= => ->.
-      by congr; rewrite /kvec /= Hep_eq /prg_enc_inner /= offunvE 1:/# /#. 
+      by congr; rewrite Hep_eq /prg_enc_inner /= KVec.initiE 1:/# /= /PRF kvec_val /=.
     case (i = 1) => Ci1.
     + rewrite Ci1 /= initiE 1:/# /= initiE 1:/# /= initiE 1:/# /= initiE 1:/# /= ifF 1:/# ifF 1:/# ifT 1:/#.
       have := Hr2; rewrite /lift_array256 tP => /(_ k _); 1: smt(); rewrite mapiE 1:/# /= => ->.
-      by congr; rewrite /kvec /= Hep_eq /prg_enc_inner /= offunvE 1:/# /#. 
+      by congr; rewrite Hep_eq /prg_enc_inner /= KVec.initiE 1:/# /= /PRF kvec_val /=.
     case (i = 2) => Ci2.
     + rewrite Ci2 /= initiE 1:/# /= initiE 1:/# /= initiE 1:/# /= initiE 1:/# /= ifF 1:/# ifT 1:/#.
       have := Hr3; rewrite /lift_array256 tP => /(_ k _); 1: smt(); rewrite mapiE 1:/# /= => ->.
-      by congr; rewrite /kvec /= Hep_eq /prg_enc_inner /= offunvE 1:/# /#. 
-    have ->: i = 3 by smt().
+      by congr; rewrite Hep_eq /prg_enc_inner /= KVec.initiE 1:/# /= /PRF kvec_val /=.
+    have ->: i = 3 by smt(kvec_val).
     rewrite /= initiE 1:/# /= initiE 1:/# /= initiE 1:/# /= initiE 1:/# /= ifT 1:/#.
     have := Hr4; rewrite /lift_array256 tP => /(_ k _); 1: smt(); rewrite mapiE 1:/# /= => ->.
-      by congr; rewrite /kvec /= Hep_eq /prg_enc_inner /= offunvE 1:/# /#. 
+    by congr; rewrite Hep_eq /prg_enc_inner /= KVec.initiE 1:/# /= /PRF kvec_val /=.
   + (* signed_bound1024_cxq sp_0 *)
     rewrite /signed_bound1024_cxq => k Hk; rewrite initiE 1:/# /=.
     case (768 <= k < 1024) => Ck4; first by smt(qE).
@@ -856,7 +907,7 @@ seq 2 0 : (#pre /\
            signed_bound_cxq epp{1} 0 256 1).
 + sp 1 0.
   wp; ecall {1} (jkem_getnoise_eta2_ph noiseseed{1} (W8.of_int 8)).
-  auto => |> &1 &2;  rewrite /prg_enc_inner=>  ??????[#]?????? result Hepp_eq Hepp_bnd;split;smt().
+  auto => |> &1 &2;  rewrite /prg_enc_inner=>  ??????[#]?????? result Hepp_eq Hepp_bnd;split;smt(kvec_val).
 
 
 (* === Step 5: NTT(sp_0) on LHS; rhat <- nttv rv on RHS. === *)
@@ -918,15 +969,17 @@ seq 2 0 : (#pre /\
          + move => ???????? rr Hrb Hrv;do split;1,2,5..:smt().
            + move => j jbl jbh.
              rewrite tP => k kb.
-             rewrite mapiE 1:/# /= initiE 1:/# /= initiE 1:/# /=.
              case (j < w{hr}) => Hj.
-             + by rewrite ifF 1:/# -Hbpv 1:/#  mapiE 1:/# /= initiE 1:/# /=.
+             +  rewrite -Hbpv; 1: smt().
+                rewrite mapiE 1:/# /= initiE 1:/# /= initiE 1:/# /=.
+                by rewrite ifF 1:/#  mapiE 1:/# /= initiE 1:/# /=.
+             rewrite mapiE 1:/# /= Array256.initiE 1:/# /= Array1024.initiE 1:/# /=.
              rewrite ifT 1:/#.
              have := Hrv; rewrite tP => Hrvk.
              have := Hrvk (256 * j + k - w{hr} * 256) _;1:smt().
              rewrite mapiE 1:/# /= => ->;do congr.
              have -> : j = w{hr} by smt().
-             by rewrite (ntt_dotp_row_eq_ntt_mmul (trmx (sampleA rho{m})) sp_0{hr} w{hr}) 1:/#;smt(getvE).
+             by rewrite (ntt_dotp_row_eq_ntt_mmul (trmx (sampleA rho{m})) sp_0{hr} w{hr}) 1:/#;smt().
           + smt().
           + rewrite /signed_bound1024_cxq => j jb; rewrite initiE 1:/# /=.
              case (j < w{hr}*256) => Hj;smt().
@@ -958,8 +1011,8 @@ seq 1 0 : (#pre /\
       rewrite nttpackv_pred  allP /= => k Hk.
       have := H0; rewrite  /pos_bound1024_cxq /#.
     + rewrite Hpkpv; congr; rewrite lift_array1024_unlift_ofipolyvec.
-      + rewrite allP => k kb /=.
-        have := decode12_vec_bnd pk{2}.`1 k _; smt().
+      + rewrite IPVec.allP => k kb /=.
+        have := decode12_vec_bnd pk{2}.`1 k _; smt(kvec_val).
       by smt().
     + by rewrite lift_array1024_nttunpackv_nttpackv.
     + move: Hthat; rewrite /pos_bound1024_cxq /signed_bound1024_cxq /bpos16 /b16 /#.
@@ -986,19 +1039,23 @@ seq 1 0 : (#{/~forall j, 0 <= j < 4 =>
   move => j Hjbl Hjbh.
   have HrsJ : lift_array256 (subarray256 result j)%Serialization =
             scale (invntt (lift_polyvec (nttpackv bp{1})).[j]%Vector) (incoeff 65536).
-  + have <- : (lift_polyvec result).[j]%Vector = lift_array256 (subarray256 result j)%Serialization
-       by rewrite /lift_polyvec offunvE 1:/# //.
-    rewrite -Hres /scale mapvE /= offunvE 1:/# //=;congr;1:smt().
-    rewrite /invnttv mapvE !offunvE 1:/# //= offunvK /vclamp ifT 1:/#.
-    by rewrite /lift_polyvec offunvK /vclamp ifT 1:/#.
+  + have <- : (lift_polyvec result).[j]%Vector = lift_array256 (subarray256 result j)%Serialization.
+       by rewrite /lift_polyvec KVec.initiE /=;1:smt(kvec_val).
+    rewrite -Hres /scale  /=  initiE /=;1:smt(kvec_val).
+    rewrite mapiE /=;1:smt(kvec_val).
+    rewrite mapiE /=;1:smt(kvec_val).
+    rewrite tP => k kb.
+    rewrite mapiE /= 1:/# mapiE /= 1:/#.
+    rewrite Zq.ComRing.mulrC;congr;congr;congr.
+    by rewrite /lift_polyvec KVec.initiE; smt(kvec_val).
 
-pose mm := offunv (fun jj =>
+pose mm := KVec.init (fun jj =>
   scale (ntt_mmul (trmx (sampleA rho{2})) (lift_polyvec (nttpackv sp_0{1}))).[jj]%Vector (incoeff 169)).
 have Hbp_polyvec : lift_polyvec (nttpackv bp{1}) = mm.
 + apply kg_loop_post_to_target => jj jjb.
-  by rewrite /mm getvE offunvE 1:/# //= Hslots 1:/#.
+  by rewrite /mm initiE;smt(kvec_val).
 
-rewrite HrsJ Hbp_polyvec /mm offunvE 1:/# //=.
+rewrite HrsJ Hbp_polyvec /mm initiE /=; 1:smt(kvec_val).
 rewrite invntt_scale.
 rewrite /scale /mul1x256 tP => k Hk.
 rewrite !mapiE //=.
@@ -1039,16 +1096,15 @@ seq 1 0 : (#{/~forall j, 0 <= j < 4 =>
 + have H := polyvec_add_corr_avx 1 1 _ _ => //.
   ecall{1} (H (lift_array1024 bp{1}) (lift_array1024 ep{1})).
   auto => |> &1 &2 ?? Hpkv Hpkb Hkv Hkb ; rewrite /prg_enc_inner => [#] Hrv Hep Hepp Hmb Hepb Heppb Hrvv Hspb  Hmk Hbpb Hvv Hvb result Hresbnd Hresk.
-  apply eq_vectorP => j Hj.
-  rewrite /lift_polyvec offunvE 1:/# /=.
-  rewrite /subarray256 /lift_array256 tP => k kb.
-  rewrite mapiE 1:/# /= initiE 1:/# /= Hresk 1:/# polyvecD /Vector.(+) offunvE 1:/# /=.
-  rewrite offunvE 1:/# /= mapiE 1:/# /= mapiE 1:/# /=.
-  rewrite /(&+) map2iE 1:/# /= mapiE 1:/# /= initiE 1:/# /=;congr.
-  have := Hmk j _; first by smt().
-  rewrite /lift_array256 tP => /(_ k _); first by smt().
-  rewrite mapiE 1:/# /= initiE 1:/# /= => ->.
-  by rewrite /invnttv mapvE offunvE;1: smt().
+  apply KVec.tP => j Hj.
+  have Hj3 : 0 <= j < 4 by smt(kvec_val).
+  rewrite polyvec_addE 1:/# invnttvE 1:/# -(Hmk j Hj3).
+  rewrite /lift_polyvec !KVec.initiE 1,2:/# /=.
+  rewrite /lift_array256 /subarray256 tP => k kb.
+  rewrite /(&+) map2iE 1:/# /= mapiE 1:/# /= mapiE 1:/# /= mapiE 1:/# /= initiE 1:/# /= initiE 1:/# /= initiE 1:/# /=.
+  have Hjk : 0 <= 256 * j + k < 1024 by smt(kvec_val).
+  rewrite Hresk 1:/#.
+  by rewrite /lift_array1024 mapiE 1:/# mapiE 1:/#.
 
 (* === Step 11: v += epp. === *)
 seq 1 0 : (#{/~lift_array256 v{1} =
@@ -1082,25 +1138,34 @@ seq 1 0 : (#{/~lift_array256 v{1} =
   split;1:by  move : Hkb;rewrite /pos_bound256_cxq /signed_bound_cxq; smt(qE).
   move => ? result Hresbnd Hresk.
   rewrite /(&+) tP => k0 kb.
-  rewrite map2iE 1:/# mapiE //=.
-  rewrite /lift_array256 mapiE //=.
-  have  : lift_array256 k{1} = decompress_poly 1 (decode1 m{2}) by smt().
-  rewrite tP => Hk_eq.
-  have := Hk_eq k0 kb;rewrite /decompress_poly (Array256.mapiE (decompress 1)) 1:/# => <-.
-  rewrite map2E initiE 1:/# /= mapiE 1:/# /= Hresk 1:/#;congr.
-  rewrite Hvv /(&+) map2E initiE 1:/# /=;congr.
-  by rewrite  /lift_array256 !mapiE //=.
+  rewrite !map2iE 1,2:/# /=.
+  have ->: (lift_array256 result).[k0]
+         = (lift_array256 v{1}).[k0] + (lift_array256 k{1}).[k0].
+  + by rewrite {1}/lift_array256 mapiE 1:/# /= Hresk 1:/#.
+  by rewrite Hvv Hkv /(&+) !map2iE 1,2:/# /=.
 
 (* === Step 13: bp reduce. === *)
 seq 1 0 : (#{/~signed_bound1024_cxq bp{1} 0 1024 2}pre /\
            pos_bound1024_cxq bp{1} 0 1024 2).
 + ecall{1} (polyvec_reduce_corr_avx (lift_array1024 bp{1})).
   auto => |>  &1 &2 ?? Hpkv Hpkb Hkv Hkb ; rewrite /prg_enc_inner => [#] Hrv Hep Hepp Hmb Hepb Heppb Hrvv Hspb Hbpv Hbpb Hvv Hvb result Hresbnd Hresk.
-  rewrite /lift_polyvec eq_vectorP => i ib.
-  rewrite offunvE //= tP => k kb.
-  have := Hbpv; rewrite eq_vectorP => Hbpk.
-  have := Hbpk i ib; rewrite  offunvE 1:/# /= tP => <-;1:smt().
-  by rewrite !subliftsub 1..4:/# -Hresbnd mapiE 1:/# /=.
+  rewrite /lift_polyvec tP => i ib.
+  rewrite initiE 1:/# /= initiE /=;  1:smt(kvec_val).
+  rewrite tP => k kb.
+  rewrite !subliftsub; 1..2:smt(kvec_val).
+  rewrite -Hresbnd mapiE 1:/# /= mapiE /=;1:smt(kvec_val).
+  move : Hbpv; rewrite tP => Hpbv.
+  have := Hpbv i _; 1:smt(kvec_val).
+  rewrite initiE 1:/# /= initiE 1:/# /= tP => Hpbvk.
+  have := Hpbvk k _;1:smt().
+  rewrite mapiE 1:/# mapiE 1:/# /= /subarray256  Array256.initiE 1:/# /= => ->.
+  congr;congr.
+  + do congr.
+    + rewrite /lift_polyvec tP => kk kkb.
+      rewrite initiE 1:/# /= initiE 1:/# /= tP => jj jjb.
+      by rewrite !mapiE 1,2:/# /= initiE 1:/# /= initiE 1:/# /=.
+    + rewrite /lift_polyvec initiE 1:/# /= initiE 1:/# /= tP => kk jjb.
+      by rewrite !mapiE 1,2:/# /= initiE 1:/# /= initiE 1:/# /=.
 
 (* === Step 14: v reduce. === *)
 seq 1 0 : (#{/~signed_bound_cxq v{1} 0 256 3}pre /\
@@ -1108,7 +1173,7 @@ seq 1 0 : (#{/~signed_bound_cxq v{1} 0 256 3}pre /\
 + ecall{1} (poly_reduce_corr_avx (lift_array256 v{1})).
   auto =>  |> &1 &2 ?? Hpkv Hpkb Hkv Hkb ; rewrite /prg_enc_inner => [#] Hrv Hep Hepp Hmb Hepb Heppb Hrvv Hspb Hbpv Hbpb Hvv Hvb result Hresbnd Hresk.
     rewrite  tP => k kb.
-  have := Hbpv; rewrite eq_vectorP => Hbpk.
+  have := Hbpv; rewrite tP => Hbpk.
   rewrite -Hresbnd mapiE 1:/# /=.
   by rewrite -Hbpb; rewrite  mapiE 1:/# /=.
 
@@ -1116,36 +1181,44 @@ seq 1 0 : (#{/~signed_bound_cxq v{1} 0 256 3}pre /\
      TODO 1024: compress widths are 11 (c1) and 5 (c2). *)
 wp; ecall {1} (i_poly_compress_corr v{1}).
 wp; ecall {1} (polyvec_compress_avx2_corr bp{1}).
-auto =>  |>  &1 &2 ?? Hpkv Hpkb Hkv Hkb; rewrite /prg_enc_inner => [#] Hrv Hep Hepp Hmb Hepb Heppb Hrvv Hspb Hbpv Hvv Hvb Hbpb result Hresv result0 Hres0; split.
+auto =>  |>  &1 &2 ?? Hpkv Hpkb Hkv Hkb; rewrite /prg_enc_inner => [#] Hrv Hep Hepp Hmb Hepb Heppb Hrvv Hspb Hbpv Hvv Hvb Hbpb result Hresv result0 Hres0.
+have Hbnd : 32 * Parameters.du * Parameters.kvec = 1408 by smt(Parameters.param_sets kvec_val).
+have Hdu : Parameters.du = 11 by smt(Parameters.param_sets kvec_val).
+have Hdv : Parameters.dv = 5 by smt(Parameters.param_sets kvec_val).
+split.
 + rewrite tP => k kn.
-  rewrite initiE 1:/# /= initiE 1:/# /= initiE 1:/# /= ifF 1:/# initiE 1:/# /= ifT 1:/#.
+  rewrite initiE 1:/# /= initiE 1:/# /= initiE /=;1:smt(Parameters.param_sets kvec_val).
+  rewrite ifF 1:/# initiE 1:/# /= ifT 1:/#.
   have := Hresv; rewrite tP => Hresvk.
+  rewrite Hbnd in kn.
   have := Hresvk k kn; rewrite initiE 1:/# /= => ->.
   rewrite /encode11_vec get_of_list 1:/# /=;do congr;smt().
-rewrite tP => k kb;rewrite initiE 1:/# /= initiE 1:/# /= initiE 1:/# /= ifT 1:/# /= Hres0.
+rewrite tP => k kb.
+rewrite initiE 1:/# /= initiE 1:/# /= initiE /=;1:smt(Parameters.param_sets kvec_val).
+rewrite ifT 1:/# /= Hres0.
 rewrite initiE 1:/# /=;do congr;smt().
 qed.
 
 lemma mlkem_correct_enc_1_avx2 _pkp :
-  equiv [Jkem_avx2.M.__indcpa_enc ~ KPKE.enc_derand :
+  equiv [Jkem_avx2.M.__indcpa_enc ~ KPKE.encrypt :
     msgp{1} = m{2} /\ pk{1} = _pkp /\
     noiseseed{1} = coins{2} /\
-    pk{2}.`1 = Array1536.init (fun i => pk{1}.[i]) /\
+    pk{2}.`1 = BytesPKVec.init (fun i => pk{1}.[i]) /\
     pk{2}.`2 = Array32.init (fun i => pk{1}.[i+1536])
     ==>
     let (c1,c2) = res{2} in
-    c1 = Array1408.init (fun i => res{1}.[i]) /\
-    c2 = Array160.init (fun i => res{1}.[i+1408])].
+    c1 = BytesCtVec.init (fun i => res{1}.[i]) /\
+    c2 = BytesPoly.init (fun i => res{1}.[i+1408])].
 proof.
 transitivity InnerPKE_Op.enc_derand
   (msgp{1} = m{2} /\ pk{1} = _pkp /\
    noiseseed{1} = r{2} /\
-   pk{2}.`1 = Array1536.init (fun i => pk{1}.[i]) /\
+   pk{2}.`1 = BytesPKVec.init (fun i => pk{1}.[i]) /\
    pk{2}.`2 = Array32.init (fun i => pk{1}.[i+1536])
    ==>
    let (c1,c2) = res{2} in
-   c1 = Array1408.init (fun i => res{1}.[i]) /\
-   c2 = Array160.init (fun i => res{1}.[i+1408]))
+   c1 = BytesCtVec.init (fun i => res{1}.[i]) /\
+   c2 = BytesPoly.init (fun i => res{1}.[i+1408]))
   (={arg} ==> ={res}).
 + smt().
 + smt().
@@ -1158,8 +1231,8 @@ lemma mlkem_correct_kg_avx2_op :
     randomnessp{1} = coins{2}
     ==>
     let (pk,sk) = res{2} in let (t,rho) = pk in
-      sk = res{1}.`2 /\
-      t = Array1536.init (fun i => res{1}.`1.[i]) /\
+      sk = BytesPKVec.init (fun i => res{1}.`2.[i]) /\
+      t = BytesPKVec.init (fun i => res{1}.`1.[i]) /\
       rho = Array32.init (fun i => res{1}.`1.[1536+i])].
 proof.
 proc => /=.
@@ -1190,12 +1263,12 @@ seq 16 5 : (#pre /\ publicseed{1} = rho{2} /\
              s{2} = (prg_kg_inner coins{2}).`2 /\
               e{2} = (prg_kg_inner coins{2}).`3 /\
              inbuf{1} = Array33.init (fun k => if k < 32 then coins{2}.[k]
-                                               else W8.of_int kvec) /\
+                                               else W8.of_int Parameters.kvec) /\
              to_list buf{1} = SHA3_512 (to_list inbuf{1})).
   + wp; ecall {1} (sha3_512A_A33_ph inbuf{1}); auto => />.
     move => &1 &2 Hbnd r Hr; rewrite tP => k kb; rewrite initiE 1:/# /= get_setE 1:/#.
     case (k = 32) => Hk.
-    + by rewrite ifF 1:/# /kvec.
+    + by rewrite ifF 1:/# kvec_val.
     by rewrite ifT 1:/# Hbnd /#.
   sp 2 0; conseq />.
   while {1} (0 <= i{1} <= inc{1} /\ inc{1} = 4 /\
@@ -1271,7 +1344,7 @@ seq 2 1 : (#pre /\ aa{1} = nttunpackm (unlift_matrix a{2}) /\
 seq 6 0 : (#pre /\
   (forall i, 0 <= i < 4 =>
      lift_array256 (Array256.init (fun k => skpv{1}.[256*i + k])) =
-       cbd2sample (Symmetric.PRF noiseseed{1} (W8.of_int i))) /\
+       samplePolyCBD (Symmetric.PRF noiseseed{1} (W8.of_int i))) /\
   signed_bound1024_cxq skpv{1} 0 1024 1).
 + sp 1 0.
   wp.
@@ -1310,39 +1383,39 @@ seq 6 0 : (#pre /\
   ecall {1} (jkem_getnoise_4x_ph noiseseed{1} (W8.of_int 4)).
   auto => |>.
   move => &1 &2 Haab Hskpv Hskpvb result Hr1 Hr2 Hr3 Hr4 Hb1 Hb2 Hb3 Hb4.
-  have Hs2v : forall i, 0 <= i < kvec => (prg_kg_inner coins{2}).`2.[i]%Vector = cbd2sample (PRF (G_coins_ds coins{2}).`2 (W8.of_int i)).
-  + by move => i Hi; rewrite /prg_kg_inner /= offunvE 1:/# /=.
-  have He3v : forall i, 0 <= i < kvec => (prg_kg_inner coins{2}).`3.[i]%Vector = cbd2sample (PRF (G_coins_ds coins{2}).`2 (W8.of_int (i + kvec))).
-  + by move => i Hi; rewrite /prg_kg_inner /= offunvE 1:/# /=.
+  have Hs2v : forall i, 0 <= i < Parameters.kvec => (prg_kg_inner coins{2}).`2.[i] = samplePolyCBD (PRF (G_coins_ds coins{2}).`2 (W8.of_int i)).
+  + by move => i Hi; rewrite /prg_kg_inner /= KVec.initiE 1:/# /=.
+  have He3v : forall i, 0 <= i < Parameters.kvec => (prg_kg_inner coins{2}).`3.[i] = samplePolyCBD (PRF (G_coins_ds coins{2}).`2 (W8.of_int (i + Parameters.kvec))).
+  + by move => i Hi; rewrite /prg_kg_inner /= KVec.initiE 1:/# /=.
   do split.
   + (* lift_polyvec skpv = (prg_kg_inner coins).`2 *)
-    rewrite eq_vectorP => i Hi.
-    rewrite Hs2v 1:/# offunvE 1:/# /=.
-    have Hspi := Hskpv i _; first by smt().
+    apply KVec.tP => i Hi.
+    rewrite Hs2v 1:/# /lift_polyvec KVec.initiE 1:/# /=.
+    have Hspi := Hskpv i _; first by smt(kvec_val).
     rewrite tP => k Hk.
     move: Hspi; rewrite /lift_array256 /subarray256 tP => /(_ k _); first by smt().
     by rewrite !mapiE 1:/# /=.
   + (* lift_polyvec e = (prg_kg_inner coins).`3 *)
-    rewrite eq_vectorP => i Hi.
-    rewrite He3v 1:/# /PRF offunvE 1:/# /=.
+    apply KVec.tP => i Hi.
+    rewrite He3v 1:/# /PRF /lift_polyvec KVec.initiE 1:/# /=.
     rewrite /lift_array256 /subarray256 tP => k Hk.
     rewrite mapiE 1:/# /= initiE 1:/# /=.
     case (i = 0) => Ci0.
     + rewrite Ci0 /= initiE 1:/# /= initiE 1:/# /= initiE 1:/# /= initiE 1:/# /= ifF 1:/# ifF 1:/# ifF 1:/# ifT 1:/#.
       have := Hr1; rewrite /lift_array256 tP => /(_ k _); 1: smt(); rewrite mapiE 1:/# /= => ->.
-      by congr; rewrite /kvec /#.
+      by congr; rewrite kvec_val /#.
     case (i = 1) => Ci1.
     + rewrite Ci1 /= initiE 1:/# /= initiE 1:/# /= initiE 1:/# /= initiE 1:/# /= ifF 1:/# ifF 1:/# ifT 1:/#.
       have := Hr2; rewrite /lift_array256 tP => /(_ k _); 1: smt(); rewrite mapiE 1:/# /= => ->.
-      by congr; rewrite /kvec /#.
+      by congr; rewrite kvec_val /#.
     case (i = 2) => Ci2.
     + rewrite Ci2 /= initiE 1:/# /= initiE 1:/# /= initiE 1:/# /= initiE 1:/# /= ifF 1:/# ifT 1:/#.
       have := Hr3; rewrite /lift_array256 tP => /(_ k _); 1: smt(); rewrite mapiE 1:/# /= => ->.
-      by congr; rewrite /kvec /#.
-    have ->: i = 3 by smt().
+      by congr; rewrite kvec_val /#.
+    have ->: i = 3 by smt(kvec_val).
     rewrite /= initiE 1:/# /= initiE 1:/# /= initiE 1:/# /= initiE 1:/# /= ifT 1:/#.
     have := Hr4; rewrite /lift_array256 tP => /(_ k _); 1: smt(); rewrite mapiE 1:/# /= => ->.
-    by congr; rewrite /kvec /#.
+    by congr; rewrite kvec_val /#.
   (* signed_bound1024_cxq e -- from Hb1..Hb4 *)
   rewrite /signed_bound1024_cxq => k Hk; rewrite initiE 1:/# /=.
   case (768 <= k < 1024) => Ck4; first by smt(qE).
@@ -1360,7 +1433,7 @@ seq 2 2 : (#{/~s{2} = (prg_kg_inner coins{2}).`2}
             {/~signed_bound1024_cxq e{1} 0 1024 1}
             {/~forall i, 0 <= i < 4 =>
                  lift_array256 (Array256.init (fun k => skpv{1}.[256*i + k])) =
-                 cbd2sample (Symmetric.PRF noiseseed{1} (W8.of_int i))}pre /\
+                 samplePolyCBD (Symmetric.PRF noiseseed{1} (W8.of_int i))}pre /\
            s{2} = lift_polyvec (nttpackv skpv{1}) /\
            e{2} = lift_polyvec (nttpackv e{1}) /\
            pos_bound1024_cxq skpv{1} 0 1024 2 /\
@@ -1375,13 +1448,13 @@ seq 2 2 : (#{/~s{2} = (prg_kg_inner coins{2}).`2}
 
 seq 6 3 : (
   publicseed{1} = rho{2} /\
-  sk{1} = sv{2} /\
-  aux_3{1} = tv{2}); last first.
+  sv{2} = BytesPKVec.init (fun i => sk{1}.[i]) /\
+  tv{2} = BytesPKVec.init (fun i => aux_3{1}.[i])); last first.
   sp 3 0.
   while {1} (inc{1} = 4 /\ 0 <= i{1} <= 4 /\
              publicseed{1} = rho{2} /\
-             sk{1} = sv{2} /\
-             aux_3{1} = tv{2} /\
+             sv{2} = BytesPKVec.init (fun i => sk{1}.[i]) /\
+             tv{2} = BytesPKVec.init (fun i => aux_3{1}.[i]) /\
              (forall k, 0 <= k < 1536 => pk{1}.[k] = aux_3{1}.[k]) /\
              (forall k, 0 <= k < i{1}*8 => pk{1}.[1536+k] = publicseed{1}.[k]))
             (4 - i{1}).
@@ -1395,14 +1468,14 @@ seq 6 3 : (
     + rewrite ifT 1:/# /get64 /get64_direct pack8bE 1:/# initiE 1:/# /=.
       rewrite /init8 initiE 1:/# /=; congr; smt().
     rewrite ifF 1:/# /get8 /init8 initiE 1:/# /=; smt().
-  auto => /> &1  Haux3.
+  auto => |> &1 &2 pk1.
   do split; 2:smt().
   + move => k kbl kbh; rewrite initiE 1:/# /= ifT 1:/#; smt().
   move => i pk;split;1:smt().
   move => Hi_neg Hi_lo Hi_hi Hpk_low Hpk_high.
   do split.
-  + rewrite tP => k Hk; rewrite initiE 1:/# /=; smt().
-  rewrite tP => k Hk; rewrite initiE 1:/# /=; smt().
+  + rewrite tP => k Hk; rewrite initiE 1:/# /= initiE 1:/# /=; smt(kvec_val Parameters.param_sets).
+  rewrite tP => k Hk; rewrite initiE 1:/# /=; smt(kvec_val Parameters.param_sets).
 
 ecall {1} (polyvec_tobytes_corr pkpv{1}).
 ecall {1} (polyvec_tobytes_corr skpv{1}).
@@ -1423,18 +1496,17 @@ conseq (: _ ==>
   do split; 1: smt().
   move => ? rr Hrrb Hrrv rr1 Hrr1v ? Hrr1b.
   split.
-  + congr. 
-    rewrite -toipolivec_lift.
-  congr.
+  + by rewrite encode12_vec_tobytes_bridge.
   have Hrr1_lift : forall k, 0 <= k < 1024 =>
       (lift_array1024 rr1).[k] = (lift_array1024 _pk).[k] + (lift_array1024 e{1}).[k].
   + move => k Hk; rewrite -Hrr1v /lift_array1024 mapiE 1:/# /=.
     by move: (Hrrv k Hk); rewrite /lift_array1024 !mapiE 1..3:/# /=.
   have Hpoly : lift_polyvec (nttpackv rr1) =
-               (lift_polyvec (nttpackv _pk) + lift_polyvec (nttpackv e{1}))%Vector
+               (lift_polyvec (nttpackv _pk) + lift_polyvec (nttpackv e{1}))
     by apply (lift_polyvec_nttpackv_add _pk e{1} rr1 Hrr1_lift).
-  rewrite -Hmmul.
-  by have := Hpoly; rewrite -toipolivec_lift  polyvecD => <-.
+  have ->: ntt_mmul (sampleA rho{2}) (lift_polyvec (nttpackv skpv{1})) + lift_polyvec (nttpackv e{1})
+         = lift_polyvec (nttpackv rr1) by rewrite Hpoly Hmmul.
+  by rewrite encode12_vec_tobytes_bridge.
 
 conseq |>.
 
@@ -1508,7 +1580,7 @@ while {1} (
     case Hcase => [Hjlt | Hjeq].
     + rewrite (subarray256_double_init_fallthrough pkpv{hr} rr0 rr1 i{hr} j) 1,2:/#; smt().
     rewrite Hjeq.
-    have ->: subarray256%Serialization
+    have ->: subarray256
       (Array1024.init
         (fun (i_0 : int) =>
            if i{hr} * 256 <= i_0 < i{hr} * 256 + 256 then rr1.[i_0 - i{hr} * 256]
@@ -1574,19 +1646,19 @@ qed.
 (* DERIVED: original target via transitivity through InnerPKE_Op (operator
    form spec) using kg_op_eq from InnerPKE_Op. *)
 lemma mlkem_correct_kg_avx2 :
-  equiv [Jkem_avx2.M.__indcpa_keypair ~ KPKE.kg_derand :
+  equiv [Jkem_avx2.M.__indcpa_keypair ~ KPKE.keygen :
     randomnessp{1} = coins{2}
     ==>
     let (pk,sk) = res{2} in let (t,rho) = pk in
-      sk = res{1}.`2 /\
-      t = Array1536.init (fun i => res{1}.`1.[i]) /\
+      sk = BytesPKVec.init (fun i => res{1}.`2.[i]) /\
+      t = BytesPKVec.init (fun i => res{1}.`1.[i]) /\
       rho = Array32.init (fun i => res{1}.`1.[1536+i])].
 proof.
 transitivity InnerPKE_Op.kg_derand
   (randomnessp{1} = coins{2} ==>
      let (pk,sk) = res{2} in let (t,rho) = pk in
-       sk = res{1}.`2 /\
-       t = Array1536.init (fun i => res{1}.`1.[i]) /\
+       sk = BytesPKVec.init (fun i => res{1}.`2.[i]) /\
+       t = BytesPKVec.init (fun i => res{1}.`1.[i]) /\
        rho = Array32.init (fun i => res{1}.`1.[1536+i]))
   (={arg} ==> ={res}).
 + smt().
@@ -1599,11 +1671,11 @@ qed.
 (********** TOP-LEVEL: mlkem_correct_dec for avx2 (1024) **************)
 
 lemma mlkem_correct_dec :
-  equiv [Jkem_avx2.M.__indcpa_dec ~ KPKE.dec :
-    ={sk} /\
+  equiv [Jkem_avx2.M.__indcpa_dec ~ KPKE.decrypt :
+    sk{2} = BytesPKVec.init (fun i => sk{1}.[i]) /\
     let (c1,c2) = cph{2} in
-      c1 = Array1408.init (fun i => ct{1}.[i]) /\
-      c2 = Array160.init (fun i => ct{1}.[1408+i])
+      c1 = BytesCtVec.init (fun i => ct{1}.[i]) /\
+      c2 = BytesPoly.init (fun i => ct{1}.[1408+i])
     ==>
     res{1} = res{2}].
 proof.
@@ -1617,7 +1689,12 @@ swap {1} 6 -4.
 seq 2 3 : (#pre /\ u{2} = lift_polyvec bp{1} /\
            signed_bound1024_cxq bp{1} 0 1024 2).
 + wp; ecall{1}(polyvec_decompress_corr (Array1408.init (fun (i : int) => ct{1}.[0 + i]))).
-  auto => /> /#.
+  auto => />.
+  move => &1 result Hb Hr.
+  have Hdu : Parameters.du = 11 by smt(Parameters.param_sets kvec_val).
+  split.
+  + by rewrite decode_vec_c1_bridge Hdu Hr.
+  move: Hb; rewrite /pos_bound1024_cxq /signed_bound1024_cxq /bpos16 /b16 /#.
 
 swap {2} [2..3] -1.
 swap {1} 2 -1.
@@ -1627,17 +1704,27 @@ swap {1} [4..5] -2.
 seq 3 2 : (#{/~ct{1}}pre /\ v{2} = lift_array256 v{1} /\
            signed_bound_cxq v{1} 0 256 1).
 + wp; ecall{1}(poly_decompress_corr (Array160.init (fun (i : int) => ct{1}.[1408 + i]))).
-  auto => /> /#.
+  auto => />.
+  move => &1 Hbp result Hr Hb.
+  have Hdv : Parameters.dv = 5 by smt(Parameters.param_sets kvec_val).
+  split.
+  + by rewrite decode_poly_c2_bridge Hdv Hr.
+  move: Hb; rewrite /pos_bound256_cxq /signed_bound_cxq /bpos16 /b16 /#.
 
 swap {1} 2 -1.
 swap {1} 3 -2.
 
 (* Step 3: frombytes sk -> skpv *)
-seq 1 3 : (#pre /\ lift_array1024 skpv{1} = nttunpackv (map incoeff (decode12_vec sk{1})) /\
+seq 1 3 : (#pre /\ lift_array1024 skpv{1} = nttunpackv (Array1024.init (fun kk => incoeff (decode12_vec sk{2}).[kk])) /\
            s{2} = ofipolyvec (decode12_vec sk{2}) /\
            pos_bound1024_cxq skpv{1} 0 1024 2).
 + wp; ecall{1}(polyvec_frombytes_corr sk{1}).
-  auto => /> /#.
+  auto => />.
+  move => &1 Hbp Hv result Hr Hrb.
+  rewrite Hr; congr.
+  have ->: to_list sk{1} = to_list (Array1536.init (fun i => sk{1}.[i])).
+  + by congr; apply Array1536.tP => k Hk; rewrite initiE 1:/#.
+  apply frombytes12_decode_bridge.
 
 swap {1} 3 -2.
 
@@ -1670,7 +1757,7 @@ seq 2 0 : (#pre /\
       have := Hb i ib; smt(qE).
     + rewrite Hskpv Hs2;congr;rewrite lift_array1024_unlift_ofipolyvec.
       + rewrite allP => k kb /=.
-        have := decode12_vec_bnd sk{2} k _; smt().
+        have := decode12_vec_bnd sk{2} k _; smt(kvec_val).
       by rewrite Heqsk.
     + by rewrite lift_array1024_nttunpackv_nttpackv.
     + move : Hsk; rewrite /pos_bound1024_cxq /signed_bound1024_cxq /bpos16 /b16 /#.
